correctness/RegexCorrectness/Data/BoundedIterator.lean
@@ -26,6 +26,10 @@ theorem ext_index {bit₁ bit₂ : BoundedIterator startIdx maxIdx} (h₁ : bit�
 theorem next_toString {bit : BoundedIterator startIdx maxIdx} (h : bit.hasNext) : (bit.next h).toString = bit.toString := by
   simp [next, Iterator.next', BoundedIterator.toString]
 
+theorem byteIdx_lt_next_byteIdx {bit : BoundedIterator startIdx maxIdx} (h : bit.hasNext) : bit.pos.byteIdx < (bit.next h).pos.byteIdx := by
+  simp [next, pos, Iterator.next'_eq_next]
+  exact String.Iterator.lt_next bit.it
+
 theorem valid_of_it_valid {bit : BoundedIterator startIdx maxIdx} (v : bit.it.Valid) : bit.Valid := v.isValid
 
 theorem valid_of_valid {bit : BoundedIterator startIdx maxIdx} (v : bit.Valid) : bit.it.Valid := Iterator.Valid.of_isValid v
@@ -34,6 +38,84 @@ theorem next_valid {bit : BoundedIterator startIdx maxIdx} (h : bit.hasNext) (v 
   apply valid_of_it_valid
   simp [next, String.Iterator.next'_eq_next]
   exact (bit.valid_of_valid v).next h
+
+theorem nextn_valid {bit : BoundedIterator startIdx maxIdx} {n : Nat} (v : bit.Valid) : (bit.nextn n).Valid := by
+  induction n generalizing bit with
+  | zero => simpa [nextn] using v
+  | succ n ih =>
+    if h : bit.hasNext then
+      simp [nextn, h]
+      exact ih (bit.next_valid h v)
+    else
+      simpa [nextn, h] using v
+
+theorem next_nextn {bit : BoundedIterator startIdx maxIdx} {n : Nat} (hnext : bit.hasNext) : (bit.next hnext).nextn n = bit.nextn (n + 1) := by
+  cases n with
+  | zero => simp [nextn, hnext]
+  | succ n => simp [nextn, hnext]
+
+theorem byteIdx_le_nextn_byteIdx (bit : BoundedIterator startIdx maxIdx) (n : Nat) : bit.pos.byteIdx ≤ (bit.nextn n).pos.byteIdx := by
+  induction n generalizing bit with
+  | zero => simp [nextn]
+  | succ n ih =>
+    simp [nextn]
+    if h : bit.hasNext then
+      simp [nextn, h]
+      exact Nat.le_of_lt (Nat.lt_of_lt_of_le (byteIdx_lt_next_byteIdx h) (ih (bit.next h)))
+    else
+      simp [nextn, h]
+
+theorem nextn_toString {bit : BoundedIterator startIdx maxIdx} {n : Nat} : (bit.nextn n).toString = bit.toString := by
+  induction n generalizing bit with
+  | zero => simp [nextn]
+  | succ n ih =>
+    if h : bit.hasNext then
+      simp [nextn, h, ih, next_toString]
+    else
+      simp [nextn, h]
+
+theorem hasNext_of_nextn_hasNext {bit : BoundedIterator startIdx maxIdx} {n : Nat} (hnext : (bit.nextn n).hasNext) : bit.hasNext := by
+  have le : bit.pos.byteIdx ≤ (bit.nextn n).pos.byteIdx := bit.byteIdx_le_nextn_byteIdx n
+  have lt : (bit.nextn n).pos.byteIdx < bit.toString.endPos.byteIdx := by
+    have : (bit.nextn n).pos.byteIdx < (bit.nextn n).toString.endPos.byteIdx := by
+      simp [hasNext, Iterator.hasNext] at hnext
+      exact hnext
+    simpa [nextn_toString]
+  show decide (bit.pos.byteIdx < bit.toString.endPos.byteIdx) = true
+  simp
+  omega
+
+theorem nextn_next_eq_next_nextn {bit : BoundedIterator startIdx maxIdx} {n : Nat} (hnext : (bit.nextn n).hasNext) : (bit.nextn n).next hnext = (bit.next (hasNext_of_nextn_hasNext hnext)).nextn n := by
+  induction n generalizing bit with
+  | zero => simp [nextn]
+  | succ n ih =>
+    have hnext₀ : bit.hasNext := hasNext_of_nextn_hasNext hnext
+    simp [nextn, hnext₀] at hnext
+    have hnext₁ : (bit.next hnext₀).hasNext := hasNext_of_nextn_hasNext hnext
+    simp [nextn, hnext₀, hnext₁]
+    exact ih hnext
+
+theorem nextn_next {bit : BoundedIterator startIdx maxIdx} {n : Nat} (hnext : (bit.nextn n).hasNext) : (bit.nextn n).next hnext = bit.nextn (n + 1) := by
+  rw [nextn_next_eq_next_nextn hnext, next_nextn]
+
+theorem IsNextNOf.toString {bit bit₀ : BoundedIterator startIdx maxIdx} (h : bit.IsNextNOf bit₀) : bit.toString = bit₀.toString := by
+  have ⟨n, eq⟩ := h
+  simp [eq, nextn_toString]
+
+theorem IsNextNOf.hasNext_of_hasNext {bit bit₀ : BoundedIterator startIdx maxIdx} (h : bit.IsNextNOf bit₀) (hnext : bit.hasNext) : bit₀.hasNext := by
+  have ⟨n, eq⟩ := h
+  cases n with
+  | zero => simpa [eq] using hnext
+  | succ n =>
+    if hnext₀ : bit₀.hasNext then
+      exact hnext₀
+    else
+      simp [nextn, hnext₀] at eq
+      simpa [eq] using hnext
+
+theorem IsNextNOf.next {bit bit₀ : BoundedIterator startIdx maxIdx} (h : bit.IsNextNOf bit₀) (hnext : bit.hasNext) : (bit.next hnext).IsNextNOf bit₀ := by
+  have ⟨n, eq⟩ := h
+  exact ⟨n + 1, by simp [eq, nextn_next]⟩
 
 def ValidFor (l r : List Char) (bit : BoundedIterator startIdx maxIdx) : Prop := bit.it.ValidFor l r
 
